extract `wf_auto2` into `wftactics.v`

matching-logic/src/Theories/Definedness_Syntax.v
@@ -14,7 +14,7 @@
  From Coq.Unicode Require Import Utf8.
  From Coq.micromega Require Import Lia.
  
- From MatchingLogic Require Import Syntax NamedAxioms DerivedOperators.
+ From MatchingLogic Require Import Syntax NamedAxioms DerivedOperators IndexManipulation.
  From MatchingLogic.Utils Require Import stdpp_ext.
  
  From stdpp Require Import base fin_sets sets propset proof_irrel option list.
@@ -166,4 +166,91 @@ Section definedness.
 
   Definition theory := theory_of_NamedAxioms named_axioms.
 
-  End definedness.
+
+
+  (* defined, total, subseteq, equal, in *)
+  Lemma bevar_subst_defined ψ (wfcψ : well_formed_closed ψ) x ϕ :
+    bevar_subst (patt_defined ϕ) ψ x = patt_defined (bevar_subst ϕ ψ x).
+  Proof. unfold patt_defined. cbn. auto. Qed.
+  Lemma bsvar_subst_defined ψ (wfcψ : well_formed_closed ψ) x ϕ :
+    bsvar_subst (patt_defined ϕ) ψ x = patt_defined (bsvar_subst ϕ ψ x).
+  Proof. unfold patt_defined. cbn. auto. Qed.
+
+  #[global]
+   Instance Unary_defined : Unary patt_defined :=
+    {| unary_bevar_subst := bevar_subst_defined ;
+       unary_bsvar_subst := bsvar_subst_defined ;
+    |}.
+  
+
+  Lemma bevar_subst_total ψ (wfcψ : well_formed_closed ψ) x ϕ :
+    bevar_subst (patt_total ϕ) ψ x = patt_total (bevar_subst ϕ ψ x).
+  Proof. unfold patt_total. simpl_bevar_subst. reflexivity. Qed.
+  
+  Lemma bsvar_subst_total ψ (wfcψ : well_formed_closed ψ) x ϕ :
+    bsvar_subst (patt_total ϕ) ψ x = patt_total (bsvar_subst ϕ ψ x).
+  Proof. unfold patt_total. simpl_bsvar_subst. reflexivity. Qed.
+
+  #[global]
+   Instance Unary_total : Unary patt_total :=
+    {| unary_bevar_subst := bevar_subst_total ;
+       unary_bsvar_subst := bsvar_subst_total ;
+    |}.
+  
+  
+  Lemma bevar_subst_equal ψ (wfcψ : well_formed_closed ψ) x ϕ₁ ϕ₂ :
+    bevar_subst (patt_equal ϕ₁ ϕ₂) ψ x = patt_equal (bevar_subst ϕ₁ ψ x) (bevar_subst ϕ₂ ψ x).
+  Proof. unfold patt_equal. simpl_bevar_subst. reflexivity. Qed.
+
+  Lemma bsvar_subst_equal ψ (wfcψ : well_formed_closed ψ) x ϕ₁ ϕ₂ :
+    bsvar_subst (patt_equal ϕ₁ ϕ₂) ψ x = patt_equal (bsvar_subst ϕ₁ ψ x) (bsvar_subst ϕ₂ ψ x).
+  Proof. unfold patt_equal. simpl_bsvar_subst. reflexivity. Qed.
+
+  #[global]
+   Instance Binary_equal : Binary patt_equal :=
+    {| binary_bevar_subst := bevar_subst_equal ;
+       binary_bsvar_subst := bsvar_subst_equal ;
+    |}.
+  
+  Lemma bevar_subst_subseteq ψ (wfcψ : well_formed_closed ψ) x ϕ₁ ϕ₂ :
+    bevar_subst (patt_subseteq ϕ₁ ϕ₂) ψ x = patt_subseteq (bevar_subst ϕ₁ ψ x) (bevar_subst ϕ₂ ψ x).
+  Proof. unfold patt_subseteq. simpl_bevar_subst. reflexivity. Qed.
+
+  Lemma bsvar_subst_subseteq ψ (wfcψ : well_formed_closed ψ) x ϕ₁ ϕ₂ :
+    bsvar_subst (patt_subseteq ϕ₁ ϕ₂) ψ x = patt_subseteq (bsvar_subst ϕ₁ ψ x) (bsvar_subst ϕ₂ ψ x).
+  Proof. unfold patt_subseteq. simpl_bsvar_subst. reflexivity. Qed.
+
+  #[global]
+   Instance Binary_subseteq : Binary patt_subseteq :=
+    {| binary_bevar_subst := bevar_subst_subseteq ;
+       binary_bsvar_subst := bsvar_subst_subseteq ;
+    |}.
+  
+
+  Lemma bevar_subst_in ψ (wfcψ : well_formed_closed ψ) x ϕ₁ ϕ₂ :
+    bevar_subst (patt_in ϕ₁ ϕ₂) ψ x = patt_in (bevar_subst ϕ₁ ψ x) (bevar_subst ϕ₂ ψ x).
+  Proof. unfold patt_in. simpl_bevar_subst. reflexivity. Qed.
+
+  Lemma bsvar_subst_in ψ (wfcψ : well_formed_closed ψ) x ϕ₁ ϕ₂ :
+    bsvar_subst (patt_in ϕ₁ ϕ₂) ψ x = patt_in (bsvar_subst ϕ₁ ψ x) (bsvar_subst ϕ₂ ψ x).
+  Proof. unfold patt_in. simpl_bsvar_subst. reflexivity. Qed.
+
+  #[global]
+   Instance Binary_in : Binary patt_in :=
+    {| binary_bevar_subst := bevar_subst_in ;
+       binary_bsvar_subst := bsvar_subst_in ;
+    |}.
+
+  (* Defines ϕ₁ to be an inversion of ϕ₂ *)
+  (* ∀ x. ϕ₁ x = ∃ y. y ∧ (x ∈ ϕ₂ y)
+     This assumes, that bound element variables x and y do not occur in ϕ₁ and ϕ₂ *)
+     Definition patt_eq_inversion_of ϕ₁ ϕ₂
+     := patt_forall
+          (patt_equal
+             (patt_app (nest_ex ϕ₁) (patt_bound_evar 0))
+             (patt_exists (patt_and (patt_bound_evar 0)
+                                    (patt_in (patt_bound_evar 1)
+                                             (patt_app (nest_ex (nest_ex ϕ₂)) (patt_bound_evar 0)))))).
+ 
+
+End definedness.
