matching-logic/src/wftactics.v
@@ -1,0 +1,147 @@
+From Coq Require Import ssreflect ssrfun ssrbool.
+Set Implicit Arguments.
+Unset Strict Implicit.
+Unset Printing Implicit Defensive.
+
+From stdpp Require Import countable infinite.
+From stdpp Require Import pmap gmap mapset fin_sets propset.
+Require Import stdpp_ext.
+
+From MatchingLogic Require Import Utils.extralibrary Syntax.
+
+Ltac wf_auto2 := unfold is_true in *;
+repeat (try assumption; try (solve [wf_auto]);
+match goal with
+| [ |- ?H -> ?G ]
+  => intro
+
+| [ |- size' (evar_open _ _ _) < _ ]
+  => rewrite evar_open_size'
+
+| [ |- size' (svar_open _ _ _) < _ ]
+  => rewrite svar_open_size'
+
+| [ |- size' _ < size' (patt_app _ _) ]
+  => simpl; lia
+
+| [ |- size' _ < size' (patt_imp _ _) ]
+  => simpl; lia
+
+| [ |- size' _ < size' (patt_exists _) ]
+  => simpl; lia
+
+| [ |- well_formed (patt_imp ?p ?q) = true]
+  => apply well_formed_imp
+
+| [ |- well_formed (patt_app ?p ?q) = true]
+  => apply well_formed_app
+
+| [ H : well_formed (patt_app ?p ?q) = true |- _]
+  => assert (well_formed p = true);
+    [eapply well_formed_app_proj1; eassumption|];
+    assert ( well_formed q = true);
+    [eapply well_formed_app_proj2; eassumption|];
+    clear H
+
+| [ H : well_formed (patt_imp ?p ?q) = true |- _]
+  => assert (well_formed p = true);
+    [eapply well_formed_imp_proj1; eassumption|];
+    assert ( well_formed q = true);
+    [eapply well_formed_imp_proj2; eassumption|];
+    clear H
+
+| [ |- well_formed (free_evar_subst ?phi ?p ?E) = true ]
+  => apply well_formed_free_evar_subst
+
+| [ |- ?x ∉ ?E ]
+  => progress simpl
+
+| [ |- ?x ∉ free_evars (free_evar_subst _ _ _) ]
+  => eapply not_elem_of_larger_impl_not_elem_of;
+     [apply free_evars_free_evar_subst|]
+
+| [frx: ?x ∉ _ |- ?x <> ?E ]
+  => clear -frx; set_solver
+
+| [frx: ?x ∉ _ |- ?x ∉ ?E ]
+  => clear -frx; set_solver
+
+| [ |- well_formed (evar_open _ _ _) = true]
+  => apply wf_evar_open_from_wf_ex
+
+| [ |- well_formed (subst_ctx _ _) = true]
+  => apply wf_sctx
+
+  (* fallback *)
+| [ |- well_formed _ = true]
+  => unfold well_formed, well_formed_closed in *; simpl in *;
+     destruct_and?; split_and?
+
+| [ |- well_formed_positive (free_evar_subst _ _ _) = true ]
+  => apply wfp_free_evar_subst
+
+| [H: well_formed_positive (patt_exists _) = true |- _]
+  => simpl in H
+
+| [H: well_formed_closed_mu_aux (patt_exists _) _ = true |- _]
+  => simpl in H
+
+| [H: well_formed_closed_ex_aux (patt_exists _) _ = true |- _]
+  => simpl in H
+
+| [ |- well_formed_closed_mu_aux (free_evar_subst _ _ _) _ = true]
+  => apply wfc_mu_free_evar_subst
+
+| [ |- well_formed_closed_ex_aux (free_evar_subst _ _ _) _ = true]
+  => apply wfc_ex_free_evar_subst_2; simpl
+
+| [ |- well_formed_positive (bsvar_subst _ _ _) = true ]
+  => apply wfp_bsvar_subst
+
+| [ |- well_formed_positive _ = true ]
+  => progress (simpl; split_and?)
+
+| [ |- no_negative_occurrence_db_b _ (free_evar_subst _ _ _) = true ]
+  => apply free_evar_subst_preserves_no_negative_occurrence
+
+| [ |- well_formed_closed_mu_aux (bsvar_subst _ _ _) _ = true ]
+  => apply wfc_mu_aux_bsvar_subst
+
+| [ |- well_formed_closed_ex_aux (bsvar_subst _ _ _) _ = true ]
+  => apply wfc_ex_aux_bsvar_subst
+
+| [ |- svar_has_negative_occurrence _ (svar_open _ _ _) = false] =>
+  unfold svar_open; apply svar_hno_bsvar_subst
+
+|[ |- context C [ svar_quantify ?X ?n (svar_open ?n ?X _) ] ]
+  => rewrite svar_quantify_svar_open
+
+| [ |- well_formed_closed_mu_aux (svar_open _ _ _) _ = true] =>
+  unfold svar_open; apply wfc_mu_aux_bsvar_subst
+
+| [ |- well_formed_closed_ex_aux (svar_open _ _ _) _ = true] =>
+  unfold svar_open; apply wfc_ex_aux_bsvar_subst
+
+| [ |- no_negative_occurrence_db_b _ _ = true ]
+  => solve [unfold well_formed in *; simpl in *; destruct_and!; assumption]
+
+| [ |- no_negative_occurrence_db_b _ (free_evar_subst _ _ _) = true ]
+  => apply free_evar_subst_preserves_no_negative_occurrence
+
+(* last option for [svar_has_negative_occurrence] *)
+| [ |- svar_has_negative_occurrence _ _ = false ]
+  => apply svar_hno_false_if_fresh
+
+| [ |- svar_is_fresh_in _ _ ]
+  => unfold svar_is_fresh_in
+
+  (* last option for well_formed_closed_ex_aux: try decreasing n *)
+| [ |- well_formed_closed_ex_aux ?p (S ?n) = true ]
+  => eapply well_formed_closed_ex_aux_ind with (ind_evar1 := n);[lia|]
+
+  (* last option for well_formed_closed_mu_aux: try decreasing n *)
+| [ |- well_formed_closed_mu_aux ?p (S ?n) = true ]
+  => eapply well_formed_closed_mu_aux_ind with (ind_svar1 := n);[lia|]
+
+end; unfold is_true in *
+).
